coq/NNRSimp/Lang/NNRSimpEq.v
@@ -1,0 +1,241 @@
+(*
+ * Copyright 2015-2016 IBM Corporation
+ *
+ * Licensed under the Apache License, Version 2.0 (the "License");
+ * you may not use this file except in compliance with the License.
+ * You may obtain a copy of the License at
+ *
+ * http://www.apache.org/licenses/LICENSE-2.0
+ *
+ * Unless required by applicable law or agreed to in writing, software
+ * distributed under the License is distributed on an "AS IS" BASIS,
+ * WITHOUT WARRANTIES OR CONDITIONS OF ANY KIND, either express or implied.
+ * See the License for the specific language governing permissions and
+ * limitations under the License.
+ *)
+
+Require Import String.
+Require Import List.
+Require Import Compare_dec.
+Require Import Equivalence.
+Require Import Morphisms.
+Require Import Setoid.
+Require Import EquivDec.
+Require Import Program.
+Require Import Utils.
+Require Import CommonRuntime.
+Require Import NNRSimp.
+Require Import NNRSimpNorm.
+Require Import NNRSimpEval.
+
+
+Section NNRSimpEq.
+  (* Equivalence for nnrs_imp *)
+
+  Local Open Scope nnrs_imp_scope.
+
+  Context {fruntime:foreign_runtime}.
+
+  Definition nnrs_imp_expr_eq (e₁ e₂:nnrs_imp_expr) : Prop :=
+    forall (h:list(string*string))
+           (σc:list (string*data))
+           (dn_σc: Forall (data_normalized h) (map snd σc))
+           (σ:pd_bindings)
+           (dn_σ: forall d, In (Some d) (map snd σ) -> data_normalized h d),
+      nnrs_imp_expr_eval h σc σ e₁ = nnrs_imp_expr_eval h σc σ e₂.
+
+  Definition nnrs_imp_stmt_eq (s₁ s₂:nnrs_imp_stmt) : Prop :=
+    forall (h:list(string*string))
+           (σc:list (string*data))
+           (dn_σc: Forall (data_normalized h) (map snd σc))
+           (σ:pd_bindings)
+           (dn_σ: forall d, In (Some d) (map snd σ) -> data_normalized h d),
+      nnrs_imp_stmt_eval h σc s₁ σ = nnrs_imp_stmt_eval h σc s₂ σ.
+  
+  Definition nnrs_imp_eq (si₁ si₂:nnrs_imp) : Prop :=
+    forall (h:list(string*string))
+           (σc:list (string*data))
+           (dn_σc: Forall (data_normalized h) (map snd σc)),
+      nnrs_imp_eval h σc si₁ = nnrs_imp_eval h σc si₂.
+
+  Global Instance nnrs_imp_expr_equiv : Equivalence nnrs_imp_expr_eq.
+  Proof.
+    unfold nnrs_imp_expr_eq. 
+    constructor; red; intros.
+    - reflexivity.
+    - symmetry; eauto.
+    - rewrite H; eauto. 
+  Qed.
+
+  Global Instance nnrs_imp_stmt_equiv : Equivalence nnrs_imp_stmt_eq.
+  Proof.
+    unfold nnrs_imp_stmt_eq. 
+    constructor; red; intros.
+    - reflexivity.
+    - symmetry; eauto.
+    - rewrite H; eauto. 
+  Qed.
+
+  Global Instance nnrs_imp_equiv : Equivalence nnrs_imp_eq.
+  Proof.
+    unfold nnrs_imp_eq. 
+    constructor; red; intros.
+    - reflexivity.
+    - symmetry; eauto.
+    - rewrite H; eauto. 
+  Qed.
+
+  Section proper.
+
+    Global Instance NNRSimpGetConstant_proper v :
+      Proper nnrs_imp_expr_eq (NNRSimpGetConstant v).
+    Proof.
+      unfold Proper, respectful, nnrs_imp_expr_eq; trivial.
+    Qed.
+
+    Global Instance NNRSimpVar_proper v :
+      Proper nnrs_imp_expr_eq (NNRSimpVar v).
+    Proof.
+      unfold Proper, respectful, nnrs_imp_expr_eq; trivial.
+    Qed.
+
+    Global Instance NNRSimpConst_proper d :
+      Proper nnrs_imp_expr_eq (NNRSimpConst d).
+    Proof.
+      unfold Proper, respectful, nnrs_imp_expr_eq; trivial.
+    Qed.
+
+    Global Instance NNRSimpBinop_proper :
+      Proper (binary_op_eq ==> nnrs_imp_expr_eq ==> nnrs_imp_expr_eq ==> nnrs_imp_expr_eq) NNRSimpBinop.
+    Proof.
+      unfold Proper, respectful, nnrs_imp_expr_eq; intros; simpl.
+      rewrite H0, H1 by trivial.
+      apply olift2_ext; intros.
+      apply H
+      ; eapply nnrs_imp_expr_eval_normalized; eauto.
+    Qed.
+
+    Global Instance NNRSimpUnop_proper :
+      Proper (unary_op_eq ==> nnrs_imp_expr_eq ==> nnrs_imp_expr_eq) NNRSimpUnop.
+    Proof.
+      unfold Proper, respectful, nnrs_imp_expr_eq; intros; simpl.
+      rewrite H0 by trivial.
+      apply olift_ext; intros.
+      apply H
+      ; eapply nnrs_imp_expr_eval_normalized; eauto.
+    Qed.
+
+    Global Instance NNRSimpGroupBy_proper s ls :
+      Proper (nnrs_imp_expr_eq ==> nnrs_imp_expr_eq) (NNRSimpGroupBy s ls).
+    Proof.
+      unfold Proper, respectful, nnrs_imp_expr_eq; intros; simpl.
+      rewrite H; trivial.
+    Qed.
+
+    Global Instance NNRSimpSeq_proper :
+      Proper (nnrs_imp_stmt_eq ==> nnrs_imp_stmt_eq ==> nnrs_imp_stmt_eq) NNRSimpSeq.
+    Proof.
+      unfold Proper, respectful, nnrs_imp_stmt_eq; intros; simpl.
+      rewrite H by trivial.
+      apply olift_ext; intros.
+      apply H0; trivial.
+      eapply nnrs_imp_stmt_eval_normalized; eauto.
+    Qed.
+
+    Global Instance NNRSimpAssign_proper v :
+      Proper (nnrs_imp_expr_eq ==> nnrs_imp_stmt_eq) (NNRSimpAssign v).
+    Proof.
+      unfold Proper, respectful, nnrs_imp_stmt_eq; intros; simpl.
+      rewrite H; trivial.
+    Qed.
+
+    Global Instance NNRSimpLet_proper v :
+      Proper (lift2P nnrs_imp_expr_eq ==> nnrs_imp_stmt_eq ==> nnrs_imp_stmt_eq) (NNRSimpLet v).
+    Proof.
+      unfold Proper, respectful, nnrs_imp_stmt_eq; intros; simpl.
+      unfold lift2P in H.
+      destruct x; destruct y; try contradiction; trivial.
+      - rewrite H; eauto 2.
+        apply olift_ext; simpl; intros ? eqq.
+        rewrite H0; trivial; simpl.
+        apply some_lift in eqq.
+        destruct eqq as [???]; subst.
+        intuition.
+        invcs H2; eauto.
+      - rewrite H0; trivial; simpl.
+        intuition; try discriminate.
+    Qed.
+
+    Global Instance NNRSimpLet_none_proper v :
+      Proper (nnrs_imp_stmt_eq ==> nnrs_imp_stmt_eq) (NNRSimpLet v None).
+    Proof.
+      apply NNRSimpLet_proper.
+      simpl; trivial.
+    Qed.
+
+    Global Instance NNRSimpFor_proper v :
+      Proper (nnrs_imp_expr_eq ==> nnrs_imp_stmt_eq ==> nnrs_imp_stmt_eq) (NNRSimpFor v).
+    Proof.
+      unfold Proper, respectful, nnrs_imp_stmt_eq; intros; simpl.
+      rewrite H; eauto 2.
+      apply olift_ext; simpl; intros ? eqq.
+      destruct a; trivial.
+      eapply nnrs_imp_expr_eval_normalized in eqq; eauto.
+      invcs eqq.
+      revert σ dn_σ.
+      induction l; simpl; trivial; intros σ dn_σ.
+      invcs H2.
+      rewrite H0; simpl; trivial.
+      - repeat (match_case; intros); subst.
+        apply IHl; trivial; intros.
+        eapply nnrs_imp_stmt_eval_normalized; eauto; simpl
+        ; intuition.
+        invcs H7; trivial.
+      - intuition.
+        invcs H3; trivial.
+    Qed.
+
+    Global Instance NNRSimpIf_proper :
+      Proper (nnrs_imp_expr_eq ==> nnrs_imp_stmt_eq ==> nnrs_imp_stmt_eq ==> nnrs_imp_stmt_eq) NNRSimpIf.
+    Proof.
+      unfold Proper, respectful, nnrs_imp_stmt_eq; intros; simpl.
+      rewrite H; eauto 2.
+      match_case; intros ? eqq.
+      destruct d; trivial.
+      destruct b; eauto.
+    Qed.
+
+    Global Instance NNRSimpEither_proper :
+      Proper (nnrs_imp_expr_eq ==> eq ==> nnrs_imp_stmt_eq ==> eq ==> nnrs_imp_stmt_eq ==> nnrs_imp_stmt_eq) NNRSimpEither.
+    Proof.
+      unfold Proper, respectful, nnrs_imp_stmt_eq; intros; simpl.
+      subst.
+      rewrite H; eauto 2.
+      match_case; intros ? eqq.
+      eapply nnrs_imp_expr_eval_normalized in eqq; eauto.
+      destruct d; trivial
+      ; invcs eqq.
+      - rewrite H1; eauto; simpl; intuition
+        ; invcs H4; eauto.
+      - rewrite H3; eauto; simpl; intuition
+        ; invcs H4; eauto.
+    Qed.      
+
+    Lemma NNRSImp_proper {s₁ s₂} : nnrs_imp_stmt_eq s₁ s₂ ->
+                                   forall v, nnrs_imp_eq (s₁, v) (s₂, v).
+    Proof.
+      unfold nnrs_imp_eq; intros eqq v; intros; simpl.
+      rewrite eqq; trivial.
+      simpl; intuition congruence.
+    Qed.
+    
+  End proper.
+  
+End NNRSimpEq.
+
+Notation "X ≡ᵉ Y" := (nnrs_imp_expr_eq X Y) (at level 90) : nnrs_imp. (* ≡ = \equiv *)
+
+Notation "X ≡ˢ Y" := (nnrs_imp_stmt_eq X Y) (at level 90) : nnrs_imp. (* ≡ = \equiv *)
+
+Notation "X ≡ˢⁱ Y" := (nnrs_imp_eq X Y) (at level 90) : nnrs_imp. (* ≡ = \equiv *)
+
