coq/NNRSimp/Typing/TNNRSimpEq.v
@@ -1,0 +1,412 @@
+(*
+ * Copyright 2015-2016 IBM Corporation
+ *
+ * Licensed under the Apache License, Version 2.0 (the "License");
+ * you may not use this file except in compliance with the License.
+ * You may obtain a copy of the License at
+ *
+ * http://www.apache.org/licenses/LICENSE-2.0
+ *
+ * Unless required by applicable law or agreed to in writing, software
+ * distributed under the License is distributed on an "AS IS" BASIS,
+ * WITHOUT WARRANTIES OR CONDITIONS OF ANY KIND, either express or implied.
+ * See the License for the specific language governing permissions and
+ * limitations under the License.
+ *)
+
+Require Import Equivalence.
+Require Import Morphisms.
+Require Import Setoid.
+Require Import EquivDec.
+Require Import Program.
+Require Import List.
+Require Import String.
+Require Import Utils.
+Require Import CommonSystem.
+Require Import NNRSimp.
+Require Import NNRSimpNorm.
+Require Import NNRSimpUsage.
+Require Import NNRSimpEval.
+Require Import NNRSimpEq.
+Require Import TNNRSimp.
+
+Section TNNRSimpEq.
+  Local Open Scope nnrs_imp.
+
+  Context {m:basic_model}.
+
+  Definition tnnrs_imp_expr_rewrites_to (e₁ e₂:nnrs_imp_expr) : Prop :=
+    forall (Γc:tbindings) (Γ : pd_tbindings) (τ:rtype),
+      [ Γc ; Γ  ⊢ e₁ ▷ τ ] ->
+      [ Γc ; Γ  ⊢ e₂ ▷ τ ] 
+      /\ (forall (σc:bindings),
+             bindings_type σc Γc ->
+             forall (σ:pd_bindings),
+               pd_bindings_type σ Γ ->
+               nnrs_imp_expr_eval brand_relation_brands  σc σ e₁
+               = nnrs_imp_expr_eval brand_relation_brands  σc σ e₂).
+
+  Definition tnnrs_imp_stmt_rewrites_to (s₁ s₂:nnrs_imp_stmt) : Prop :=
+    forall (Γc:tbindings) (Γ : pd_tbindings) ,
+      [ Γc ; Γ  ⊢ s₁ ] ->
+      [ Γc ; Γ  ⊢ s₂ ] 
+      /\ (forall (σc:bindings),
+             bindings_type σc Γc ->
+             forall (σ:pd_bindings),
+               pd_bindings_type σ Γ ->
+               nnrs_imp_stmt_eval brand_relation_brands  σc s₁ σ
+               = nnrs_imp_stmt_eval brand_relation_brands  σc s₂ σ).
+
+  Definition tnnrs_imp_rewrites_to (si₁ si₂:nnrs_imp) : Prop :=
+    forall (Γc:tbindings) (τ:rtype) ,
+      [ Γc ⊢ si₁ ▷ τ  ] ->
+      [ Γc ⊢ si₂ ▷ τ  ] 
+      /\ (forall (σc:bindings),
+             bindings_type σc Γc ->
+             nnrs_imp_eval brand_relation_brands  σc si₁
+             = nnrs_imp_eval brand_relation_brands  σc si₂).
+
+  Notation "e1 ⇒ᵉ e2" := (tnnrs_imp_expr_rewrites_to e1 e2) (at level 80) : nnrs_imp.
+  Notation "s1 ⇒ˢ s2" := (tnnrs_imp_stmt_rewrites_to s1 s2) (at level 80) : nnrs_imp.
+  Notation "si1 ⇒ˢⁱ si2" := (tnnrs_imp_rewrites_to si1 si2) (at level 80) : nnrs_imp.
+
+  (* They are all preorders *)
+  Global Instance tnnrs_imp_expr_rewrites_to_pre : PreOrder tnnrs_imp_expr_rewrites_to.
+  Proof.
+    unfold tnnrs_imp_expr_rewrites_to.
+    constructor; red.
+    - intuition.
+    - intros x y z Hx Hy; intros ? ? ? typx.
+      specialize (Hx _ _ _ typx).
+      destruct Hx as [typy Hx].
+      specialize (Hy _ _ _ typy).
+      destruct Hy as [typz Hy].
+      split; trivial; intros.
+      rewrite Hx, Hy; trivial.
+  Qed.
+
+  Global Instance tnnrs_imp_stmt_rewrites_to_pre : PreOrder tnnrs_imp_stmt_rewrites_to.
+  Proof.
+    unfold tnnrs_imp_stmt_rewrites_to.
+    constructor; red.
+    - intuition.
+    - intros x y z Hx Hy; intros ? ? typx.
+      specialize (Hx _ _ typx).
+      destruct Hx as [typy Hx].
+      specialize (Hy _ _ typy).
+      destruct Hy as [typz Hy].
+      split; trivial; intros.
+      rewrite Hx, Hy; trivial.
+  Qed.
+  
+  Global Instance tnnrs_imp_rewrites_to_pre : PreOrder tnnrs_imp_rewrites_to.
+  Proof.
+    unfold tnnrs_imp_rewrites_to.
+    constructor; red.
+    - intuition.
+    - intros x y z Hx Hy; intros ? ? typx.
+      specialize (Hx _ _ typx).
+      destruct Hx as [typy Hx].
+      specialize (Hy _ _ typy).
+      destruct Hy as [typz Hy].
+      split; trivial; intros.
+      rewrite Hx, Hy; trivial.
+  Qed.
+
+  (* An untyped equivalence + type preservation -> typed rewrite *)
+  Lemma nnrs_imp_expr_eq_rewrites_to (e₁ e₂:nnrs_imp_expr) :
+    e₁ ≡ᵉ e₂ ->
+    (forall {Γc:tbindings} {Γ:tbindings} {τ:rtype},
+        [ Γc ; Γ  ⊢ e₁ ▷ τ ] ->
+        [ Γc ; Γ  ⊢ e₂ ▷ τ ]) ->
+    e₁ ⇒ᵉ e₂.
+  Proof.
+    red; intros eqq; intros; split; eauto; intros ??? typ2.
+    apply eqq.
+    - apply Forall_map.
+      eapply bindings_type_Forall_normalized; eauto.
+    - intros ? inn.
+      eapply pd_bindings_type_in_normalized in typ2; eauto.
+  Qed.
+  
+  Lemma nnrs_imp_stmt_eq_rewrites_to (s₁ s₂:nnrs_imp_stmt) :
+    s₁ ≡ˢ s₂ ->
+    (forall {Γc:tbindings} {Γ:tbindings},
+        [ Γc ; Γ ⊢ s₁ ] ->
+        [ Γc ; Γ ⊢ s₂ ]) ->
+    s₁ ⇒ˢ s₂.
+  Proof.
+    red; intros eqq; intros; split; eauto; intros ??? typ2.
+    apply eqq.
+    - apply Forall_map.
+      eapply bindings_type_Forall_normalized; eauto.
+    - intros ? inn.
+      eapply pd_bindings_type_in_normalized in typ2; eauto.
+  Qed.
+  
+  Lemma nnrs_imp_eq_rewrites_to (si₁ si₂:nnrs_imp) :
+    si₁ ≡ˢⁱ si₂ ->
+    (forall {Γc:tbindings} {τ:rtype},
+        [ Γc ⊢ si₁ ▷ τ  ] ->
+        [ Γc ⊢ si₂ ▷ τ  ]) ->
+    si₁ ⇒ˢⁱ si₂.
+  Proof.
+    red; intros eqq; intros; split; eauto; intros.
+    apply eqq.
+    apply Forall_map.
+    eapply bindings_type_Forall_normalized; eauto.
+  Qed.
+  
+  Section proper.
+
+    Global Instance NNRSimpGetConstant_tproper v :
+      Proper tnnrs_imp_expr_rewrites_to (NNRSimpGetConstant v).
+    Proof.
+      unfold Proper, respectful, tnnrs_imp_expr_rewrites_to; intuition.
+    Qed.
+
+    Global Instance NNRSimpVar_tproper v :
+      Proper tnnrs_imp_expr_rewrites_to (NNRSimpVar v).
+    Proof.
+      unfold Proper, respectful, tnnrs_imp_expr_rewrites_to; intuition.
+    Qed.
+
+    Global Instance NNRSimpConst_tproper d :
+      Proper tnnrs_imp_expr_rewrites_to (NNRSimpConst d).
+    Proof.
+      unfold Proper, respectful, tnnrs_imp_expr_rewrites_to; intuition.
+    Qed.
+
+    Global Instance NNRSimpBinop_tproper :
+      Proper (tbinary_op_rewrites_to ==> tnnrs_imp_expr_rewrites_to ==> tnnrs_imp_expr_rewrites_to ==> tnnrs_imp_expr_rewrites_to) NNRSimpBinop.
+    Proof.
+      unfold Proper, respectful, tnnrs_imp_expr_rewrites_to.
+      intros op op' eqop e1 e1' He1 e2 e2' He2 Γc Γ τ typ.
+      invcs typ.
+      specialize (He1 _ _ _ H5).
+      destruct He1 as [typ1 He1].
+      specialize (He2 _ _ _ H6).
+      destruct He2 as [typ2 He2].
+      destruct (eqop _ _ _ H3) as [typop Hop].
+      split; [econstructor; eauto | ].
+      simpl; intros.
+      rewrite He1, He2 by trivial.
+      apply olift2_ext; intros.
+      apply Hop.
+      - eapply nnrs_imp_expr_eval_preserves_types; eauto.
+        rewrite He1; trivial.
+      -  eapply nnrs_imp_expr_eval_preserves_types; eauto.
+         rewrite He2; trivial.
+    Qed.
+
+    Global Instance NNRSimpUnop_tproper :
+      Proper (tunary_op_rewrites_to ==> tnnrs_imp_expr_rewrites_to ==> tnnrs_imp_expr_rewrites_to) NNRSimpUnop.
+    Proof.
+      unfold Proper, respectful, tnnrs_imp_expr_rewrites_to; simpl.
+      intros op op' eqop e1 e1' He1 Γc Γ τ typ.
+      invcs typ.
+      specialize (He1 _ _ _ H4).
+      destruct He1 as [typ1 He1].
+      destruct (eqop _ _ H2) as [typop Hop].
+      split; [econstructor; eauto | ].
+      simpl; intros.
+      rewrite He1 by trivial.
+      apply olift_ext; intros.
+      apply Hop.
+      eapply nnrs_imp_expr_eval_preserves_types; eauto.
+      rewrite He1; trivial.
+    Qed.
+
+    Global Instance NNRSimpGroupBy_tproper s ls :
+      Proper (tnnrs_imp_expr_rewrites_to ==> tnnrs_imp_expr_rewrites_to) (NNRSimpGroupBy s ls).
+    Proof.
+      unfold Proper, respectful, tnnrs_imp_expr_rewrites_to; simpl.
+      intros e1 e1' He1 Γc Γ τ typ.
+      invcs typ.
+      specialize (He1 _ _ _ H5).
+      destruct He1 as [typ1 He1].
+      split; [econstructor; eauto | ].
+      intros.
+      rewrite He1; trivial.
+    Qed.
+
+    Global Instance NNRSimpSeq_tproper :
+      Proper (tnnrs_imp_stmt_rewrites_to ==> tnnrs_imp_stmt_rewrites_to ==> tnnrs_imp_stmt_rewrites_to) NNRSimpSeq.
+    Proof.
+      unfold Proper, respectful, tnnrs_imp_stmt_rewrites_to; simpl.
+      intros s1 s1' Hs1 s2 s2' Hs2 Γc Γ typ.
+      invcs typ.
+      specialize (Hs1 _ _ H2).
+      destruct Hs1 as [typ1 Hs1].
+      specialize (Hs2 _ _ H3).
+      destruct Hs2 as [typ2 Hs2].
+      split; [econstructor; eauto | ].
+      intros.
+      rewrite Hs1 by trivial.
+      apply olift_ext; intros.
+      apply Hs2; trivial.
+      eapply nnrs_imp_stmt_eval_preserves_types in H1; eauto.
+    Qed.
+
+    Global Instance NNRSimpAssign_tproper v :
+      Proper (tnnrs_imp_expr_rewrites_to ==> tnnrs_imp_stmt_rewrites_to) (NNRSimpAssign v).
+    Proof.
+      unfold Proper, respectful, tnnrs_imp_stmt_rewrites_to; simpl.
+      intros e1 e1' He1 Γc Γ typ.
+      invcs typ.
+      apply He1 in H2.
+      destruct H2 as [typ1 He1'].
+      split; [econstructor; eauto | ].
+      intros.
+      rewrite He1'; trivial.
+    Qed.
+
+    Lemma NNRSimpLet_some_tproper v : 
+      forall (e₁ e₂: nnrs_imp_expr),
+        e₁ ⇒ᵉ e₂ ->
+        forall (s₁ s₂:nnrs_imp_stmt),
+          s₁ ⇒ˢ s₂ ->
+          NNRSimpLet v (Some e₁) s₁ ⇒ˢ NNRSimpLet v (Some e₂) s₂.
+    Proof.
+      intros e1 e1' He1 s2 s2' Hs2 Γc Γ typ.
+      invcs typ.
+      apply He1 in H2.
+      destruct H2 as [typ1 He1'].
+      specialize (Hs2 _ _ H4).
+      destruct Hs2 as [typ2 Hs2].
+      split; [econstructor; eauto | ].
+      simpl; intros.
+      rewrite He1' by trivial.
+      apply olift_ext; intros.
+      rewrite Hs2; trivial.
+      apply some_lift in H1.
+      destruct H1 as [? eqq1 ?]; subst.
+      eapply nnrs_imp_expr_eval_preserves_types in eqq1; eauto.
+      econstructor; simpl; eauto.
+      split; trivial; intros ? eqq2; invcs eqq2; trivial.
+    Qed.
+
+    Lemma NNRSimpLet_none_tproper v : 
+      forall (s₁ s₂:nnrs_imp_stmt),
+        s₁ ⇒ˢ s₂ ->
+        (nnrs_imp_stmt_var_usage s₁ v <> VarMayBeUsedWithoutAssignment ->
+        nnrs_imp_stmt_var_usage s₂ v <> VarMayBeUsedWithoutAssignment) ->
+        NNRSimpLet v None s₁ ⇒ˢ NNRSimpLet v None s₂.
+    Proof.
+      intros s2 s2' Hs2 Γc Γ vu typ.
+      invcs typ.
+      specialize (Hs2 _ _ H3).
+      destruct Hs2 as [typ2 Hs2].
+      split; [econstructor; eauto | ].
+      simpl; intros.
+      rewrite Hs2; trivial.
+      econstructor; simpl; eauto.
+      split; trivial; intros ? eqq2; invcs eqq2; trivial.
+    Qed.
+    
+    Global Instance NNRSimpFor_tproper v :
+      Proper (tnnrs_imp_expr_rewrites_to ==> tnnrs_imp_stmt_rewrites_to ==> tnnrs_imp_stmt_rewrites_to) (NNRSimpFor v).
+    Proof.
+      unfold Proper, respectful, tnnrs_imp_stmt_rewrites_to; simpl.
+      intros e1 e1' He1 s2 s2' Hs2 Γc Γ typ.
+      invcs typ.
+      apply He1 in H2.
+      destruct H2 as [typ1 He1'].
+      specialize (Hs2 _ _ H4).
+      destruct Hs2 as [typ2 Hs2].
+      split; [econstructor; eauto | ].
+      simpl; intros.
+      rewrite He1' by trivial.
+      apply olift_ext; intros.
+      destruct a; trivial.
+      eapply nnrs_imp_expr_eval_preserves_types in H1; eauto.
+      invcs H1; rtype_equalizer; subst.
+      clear e1 e1' typ1 He1 He1'.
+      revert σ H0.
+      induction l; simpl; trivial.
+      intros σ bt.
+      invcs H5.
+      rewrite Hs2; eauto.
+      - match_option.
+        destruct p; trivial.
+        eapply IHl; eauto.
+        eapply nnrs_imp_stmt_eval_preserves_types in eqq; eauto.
+        + invcs eqq; trivial.
+        + econstructor; simpl; eauto.
+          split; trivial; intros ? eqq2; invcs eqq2; trivial.
+      - econstructor; simpl; eauto.
+        split; trivial; intros ? eqq2; invcs eqq2; trivial.
+    Qed.
+    
+    Global Instance NNRSimpIf_tproper :
+      Proper (tnnrs_imp_expr_rewrites_to ==> tnnrs_imp_stmt_rewrites_to ==> tnnrs_imp_stmt_rewrites_to ==> tnnrs_imp_stmt_rewrites_to) NNRSimpIf.
+    Proof.
+      unfold Proper, respectful, tnnrs_imp_stmt_rewrites_to; simpl.
+      intros e1 e1' He1 s1 s1' Hs1 s2 s2' Hs2 Γc Γ typ.
+      invcs typ.
+      apply He1 in H3.
+      destruct H3 as [type He1'].
+      specialize (Hs1 _ _ H4).
+      destruct Hs1 as [typ1 Hs1].
+      specialize (Hs2 _ _ H5).
+      destruct Hs2 as [typ2 Hs2].
+      split; [econstructor; eauto | ].
+      intros.
+      rewrite He1' by trivial.
+      match_option.
+      destruct d; trivial.
+      destruct b; eauto.
+    Qed.
+
+    Global Instance NNRSimpEither_tproper :
+      Proper (tnnrs_imp_expr_rewrites_to ==> eq ==> tnnrs_imp_stmt_rewrites_to ==> eq ==> tnnrs_imp_stmt_rewrites_to ==> tnnrs_imp_stmt_rewrites_to) NNRSimpEither.
+    Proof.
+      unfold Proper, respectful, tnnrs_imp_stmt_rewrites_to; simpl.
+      intros e1 e1' He1 ? ? ? s1 s1' Hs1 ? ? ? s2 s2' Hs2 Γc Γ typ.
+      subst.
+      invcs typ.
+      apply He1 in H3.
+      destruct H3 as [type He1'].
+      specialize (Hs1 _ _ H6).
+      destruct Hs1 as [typ1 Hs1].
+      specialize (Hs2 _ _ H7).
+      destruct Hs2 as [typ2 Hs2].
+      split; [econstructor; eauto | ].
+      intros.
+      rewrite He1' by trivial.
+      match_option.
+      eapply nnrs_imp_expr_eval_preserves_types in eqq; eauto.
+      invcs eqq; rtype_equalizer; subst.
+      - rewrite Hs1; trivial.
+        econstructor; simpl; eauto.
+        split; trivial; intros ? eqq2; invcs eqq2; trivial.
+      - rewrite Hs2; trivial.
+        econstructor; simpl; eauto.
+        split; trivial; intros ? eqq2; invcs eqq2; trivial.
+    Qed.      
+
+    Lemma NNRSImp_tproper {s₁ s₂} : tnnrs_imp_stmt_rewrites_to s₁ s₂ ->
+                                    forall v,
+                                      (nnrs_imp_stmt_var_usage s₁ v <> VarMayBeUsedWithoutAssignment ->
+                                       nnrs_imp_stmt_var_usage s₂ v <> VarMayBeUsedWithoutAssignment) ->
+                                   tnnrs_imp_rewrites_to (s₁, v) (s₂, v).
+    Proof.
+      unfold tnnrs_imp_rewrites_to; intros eqq v neimpl Γc τ [ne typ].
+      eapply eqq in typ.
+      destruct typ as [typ IHs].
+      split.
+      - split; eauto.
+      - intros; simpl.
+        rewrite IHs; trivial.
+        econstructor; simpl; eauto.
+        intuition; discriminate.
+    Qed.
+    
+  End proper.
+
+End TNNRSimpEq.
+
+Notation "e1 ⇒ᵉ e2" := (tnnrs_imp_expr_rewrites_to e1 e2) (at level 80) : nnrs_imp.
+Notation "s1 ⇒ˢ s2" := (tnnrs_imp_stmt_rewrites_to s1 s2) (at level 80) : nnrs_imp.
+Notation "si1 ⇒ˢⁱ si2" := (tnnrs_imp_rewrites_to si1 si2) (at level 80) : nnrs_imp.
+
